acls without assume, and also handling revocations in acls2.fst; hiding local state in sep/counters.fst; revised model of maps and state in partialmap.fst and st/stperm.fst

src/absyn/print.fs
@@ -295,11 +295,18 @@ let freevars_to_string (fvs:freevars) =
     let f (l:set<bvar<'a,'b>>) = l |> Util.set_elements |> List.map (fun t -> strBvd t.v) |> String.concat ", " in
     Util.format2 "ftvs={%s}, fxvs={%s}" (f fvs.ftvs) (f fvs.fxvs) 
 
+let qual_to_string = function
+    | Logic -> "logic"
+    | Opaque -> "opaque"
+    | Discriminator _ -> "discriminator"
+    | Projector _ -> "projector"
+    | _ -> "other"
+let quals_to_string quals = quals |> List.map qual_to_string |> String.concat " " 
 let rec sigelt_to_string x = match x with 
-  | Sig_tycon(lid, tps, k, _, _, _, _) -> Util.format3 "type %s %s : %s" lid.str (binders_to_string " " tps) (kind_to_string k)
+  | Sig_tycon(lid, tps, k, _, _, quals, _) -> Util.format4 "%s type %s %s : %s" (quals_to_string quals) lid.str (binders_to_string " " tps) (kind_to_string k)
   | Sig_typ_abbrev(lid, tps, k, t, _, _) ->  Util.format4 "type %s %s : %s = %s" lid.str (binders_to_string " " tps) (kind_to_string k) (typ_to_string t)
   | Sig_datacon(lid, t, _, _, _) -> Util.format2 "datacon %s : %s" lid.str (typ_to_string t)
-  | Sig_val_decl(lid, t, _, _) -> Util.format2 "val %s : %s" lid.str (typ_to_string t)
+  | Sig_val_decl(lid, t, quals, _) -> Util.format3 "%s val %s : %s" (quals_to_string quals) lid.str (typ_to_string t)
   | Sig_assume(lid, f, _, _) -> Util.format2 "val %s : %s" lid.str (typ_to_string f)
   | Sig_let(lbs, _, _) -> lbs_to_string lbs
   | Sig_main(e, _) -> Util.format1 "let _ = %s" (exp_to_string e)
