src/tc/tcenv.fsi
@@ -59,6 +59,7 @@ type env = {
   lattice:lattice;               (* monad lattice *)
   generalize:bool;               (* should we generalize let bindings? *)
   letrecs:list<(lbname * typ)>   (* mutually recursive names and their types (for termination checking) *)
+  top_level:bool;                (* is this a top-level term? if so, then discharge guards *)
 }
 and solver_t = {
     init: env -> unit;
