examples/sep/counters.fst
@@ -14,55 +14,59 @@
    limitations under the License.
 *)
 module Evens
-logic type even (x:int) = x % 2 == 0
+open Heap
+open Set
+open ST
+type even (x:int) = x%2=0
 
-effect Evens (inv:heap -> Type) (fp:refs) = 
-          ST2 int (requires (fun h => On fp inv h))
-                  (ensures (fun h u h' => even u /\ On fp inv h'))
-                  (modifies fp)
+effect InvST (t:Type) (inv:(heap -> Type)) (fp:set aref) (post:(heap -> t -> heap -> Type)) =
+             ST t (fun h -> On fp inv h)
+                  (fun h i h' -> post h i h' /\ On fp inv h')
+                  (SomeRefs fp)
     
-type t = 
+type even_post (h:heap) (i:int) (h':heap) = even i
+
+
+type t =
   | Evens : inv:(heap -> Type)
-          -> fp:refs (* ghost *)
-          -> (unit -> Evens inv fp)
+          -> fp:set aref
+          -> (unit -> InvST int inv fp even_post)
           -> t
 
-opaque type inv1 (r1:ref int) (r2:ref int) (h:heap) = 
-    Perm r1 h /\ Perm r2 h /\ SelHeap h r1 = SelHeap h r2
+opaque type inv1 (r1:ref int) (r2:ref int) (h:heap) =
+           Heap.sel h r1 = Heap.sel h r2
+           /\ contains h r1
+           /\ contains h r2
 
-val mk_counter: unit 
-          -> ST2 t (requires (fun h -> True))
-                   (ensures  (fun h v h' -> 
-                             On  (Evens.fp v) (Evens_inv v) h'
-                             /\ Fresh h (Evens.fp v)))
-                   (modifies no_refs)
+val mk_counter: unit
+             -> ST t (requires (fun h -> True))
+                     (ensures  (fun h v h' ->
+                             On  (Evens.fp v) (Evens.inv v) h'
+                             /\ Heap.fresh h (Evens.fp v)))
+                     (modifies no_refs)
 let mk_counter _ =
-  let x = alloc 0 in
-  let y = alloc 0 in
-  let fp = Union (Singleton x) (Singleton y) in 
-  let evens : unit -> Evens (inv1 x y) fp = fun _ -> 
-    let rx = !x in 
-    let ry = !y in 
-    x := rx + 1;
-    y := ry + 1;
+  let x = ST.alloc 0 in
+  let y = ST.alloc 0 in
+  let evens () =
+    let rx = ST.read x in
+    let ry = ST.read y in
+    ST.write x (rx + 1);
+    ST.write y (ry + 1);
     rx + ry in
-  Evens (inv1 x y) fp evens
-    
+  Evens (inv1 x y) (Set.union (Set.singleton (Ref x)) (Set.singleton (Ref y))) evens
 
-opaque type inv2 (r:ref int) (h:heap) = Perm r h
 
-val mk_counter_2: unit 
-              -> ST2 t (requires (fun h -> True))
-                       (ensures (fun h v h' -> 
-                         On  (Evens_proj_1 v) (Evens_proj_0 v) h'
-                         /\ Fresh h (Evens_proj_1 v)))
-                              (Modifies EmptySet)
-let create2 (u:unit) = 
-  let x = ref 0 in
-  let fp = Singleton x in
-  let evens (u:unit) : evens_t (Inv2 x) fp =
-    let rx = !x in
-    x := rx + 1;
+opaque logic type inv2 (r:ref int) (h:heap) = b2t(contains h r)
+val mk_counter_2: unit
+               -> ST t (requires (fun h -> True))
+                       (ensures  (fun h v h' ->
+                         On  (Evens.fp v) (Evens.inv v) h'
+                         /\ Heap.fresh h (Evens.fp v)))
+                       (modifies no_refs)
+let mk_counter_2 _ =
+  let x = ST.alloc 0 in
+  let evens = fun _ ->
+    let rx = ST.read x in
+    ST.write x (rx + 1);
     2 * rx in
-  Evens (Inv2 x) fp evens
-    
+  Evens (inv2 x) (Set.singleton (Ref x)) evens
