lib/partialmap.fst
@@ -1,57 +1,102 @@
+module Set
+open Prims.PURE
+assume type set : Type -> Type
+
+assume val empty:      a:Type -> Tot (set a)
+assume val singleton : a:Type -> a -> Tot (set a)
+assume val union     : a:Type -> set a -> set a -> Tot (set a)
+assume val intersect : a:Type -> set a -> set a -> Tot (set a)
+assume val complement: a:Type -> set a -> Tot (set a)
+assume val mem:        a:Type -> a -> set a -> Tot bool
+assume val equal:      a:Type -> set a -> set a -> Tot bool
+
+assume MemEmpty:      forall (key:Type) (k:key).                           {:pattern mem k empty}
+                      not (mem k empty)
+
+assume MemSingleton:  forall (key:Type) (k:key) (k':key).                  {:pattern mem k (singleton k')}
+                      mem k (singleton k') == (k=k')
+
+assume MemUnion:      forall (key:Type) (s1:set key) (s2:set key) (k:key). {:pattern mem k (union s1 s2)}
+                      mem k (union s1 s2) == (mem k s1 || mem k s2)
+
+assume MemIntersect:  forall (key:Type) (s1:set key) (s2:set key) (k:key). {:pattern mem k (intersect s1 s2)}
+                      mem k (intersect s1 s2) == (mem k s1 && mem k s2)
+
+assume MemComplement: forall (key:Type) (s1:set key) (k:key).              {:pattern mem k (complement s1)}
+                      mem k (complement s1) == not(mem k s1)
+
+assume Extensional:   forall (key:Type) (s1:set key) (s2:set key).         {:pattern (equal s1 s2)}              
+                      equal s1 s2 <==> s1 == s2
+
+assume Equals:        forall (key:Type) (s1:set key) (s2:set key).         {:pattern (equal s1 s2)}              
+                      equal s1 s2 <==> (forall k.{:pattern (mem k s1); (mem k s2)} mem k s1 == mem k s2)
+
+(* derived forms *)
+let minus      (a:Type) (s1:set a) (s2:set a)  = intersect s1 (complement s2)
+opaque type Subset' (a:Type) (s1:set a) (s2:set a) = (forall (x:a).{:pattern mem x s1} mem x s1 ==> mem x s2)
+type Subset : #a:Type -> set a -> set a -> Type = 
+    fun (a:Type) (s1:set a) (s2:set a) -> Subset' a s1 s2
+
 module Map
 open Prims.PURE
+open Set
+
 assume type t : Type -> Type -> Type
-type set (a:Type) = t a bool
 assume logic val sel :       key:Type -> value:Type -> t key value -> key -> Tot value
 assume logic val upd :       key:Type -> value:Type -> t key value -> key -> value -> Tot (t key value)
 assume logic val const :     key:Type -> value:Type -> v:value -> Tot (t key value)
 assume logic val concat:     key:Type -> value:Type -> t key value -> t key value -> Tot (t key value)
 assume logic val contains:   key:Type -> value:Type -> t key value -> key -> Tot bool
 assume logic val equal:      key:Type -> value:Type -> t key value -> t key value -> Tot bool
-assume logic val intersect:  key:Type -> set key -> set key -> Tot (set key)
-assume logic val complement: key:Type -> set key -> Tot (set key)
 assume logic val restrict:   key:Type -> value:Type -> set key -> t key value -> Tot (t key value)
 
-assume SelUpd1:       forall (key:Type) (value:Type) (m:t key value) (k:key) (v:value).          {:pattern (sel (upd m k v) k)}        sel (upd m k v) k == v
-assume SelUpd2:       forall (key:Type) (value:Type) (m:t key value) (k1:key) (k2:key) (v:value).{:pattern (sel (upd m k2 v) k1)}      k2=!=k1 ==> sel (upd m k2 v) k1 == sel m k1
-assume SelConst:      forall (key:Type) (value:Type) (v:value) (k:key).                          {:pattern (sel (const v) k)}          sel (const v) k == v
-assume SelRestrict:   forall (key:Type) (value:Type) (m:t key value) (ks:set key) (k:key).       {:pattern (sel (restrict ks m) k)}    sel ks k ==> sel (restrict ks m) k == sel m k
-assume SelConcat1:    forall (key:Type) (value:Type) (m1:t key value) (m2:t key value) (k:key).  {:pattern sel (concat m1 m2) k}       contains m2 k ==> sel (concat m1 m2) k==sel m2 k
-assume SelConcat1:    forall (key:Type) (value:Type) (m1:t key value) (m2:t key value) (k:key).  {:pattern sel (concat m1 m2) k}       not(contains m2 k) ==> sel (concat m1 m2) k==sel m1 k
+assume SelUpd1:       forall (key:Type) (value:Type) (m:t key value) (k:key) (v:value).          {:pattern sel (upd m k v) k}
+                      sel (upd m k v) k == v
 
-assume InDomUpd1:     forall (key:Type) (value:Type) (m:t key value) (k:key) (v:value).          {:pattern contains (upd m k v) k}     contains (upd m k v) k
-assume InDomUpd2:     forall (key:Type) (value:Type) (m:t key value) (k1:key) (k2:key) (v:value).{:pattern contains (upd m k2 v) k1}   k2=!=k1 ==> contains (upd m k2 v) k1 == contains m k1
-assume InDomConstMap: forall (key:Type) (value:Type) (v:value) (k:key).                          {:pattern contains (const v) k}       contains (const v) k
-assume InDomConcat:   forall (key:Type) (value:Type) (m1:t key value) (m2:t key value) (k:key).  {:pattern contains (concat m1 m2) k}  contains (concat m1 m2) k==(contains m1 k || contains m2 k)
-assume InDomRestrict: forall (key:Type) (value:Type) (m:t key value) (ks:set key) (k:key).       {:pattern contains (restrict ks m) k} contains (restrict ks m) k == sel ks k
-assume ContainsConst: forall (key:Type) (value:Type) (v:value) (k:key).                          {:pattern contains (const v) k}       not (contains (const v) k)
+assume SelUpd2:       forall (key:Type) (value:Type) (m:t key value) (k1:key) (k2:key) (v:value).{:pattern sel (upd m k2 v) k1}
+                      k2=!=k1 ==> sel (upd m k2 v) k1 == sel m k1
 
-assume InInter:       forall (key:Type) (s1:set key) (s2:set key) (k:key).                       {:pattern sel (intersect s1 s2) k}    sel (intersect s1 s2) k == (sel s1 k && sel s2 k)
-assume InComplement:  forall (key:Type) (s:set key) (k:key).                                     {:pattern sel (complement s) k}       sel (complement s) k == not (sel s k)
-assume Extensional:   forall (key:Type) (value:Type) (m1:t key value) (m2:t key value).          {:pattern (equal m1 m2)}              equal m1 m2 <==> m1 == m2
-assume Equals:        forall (key:Type) (value:Type) (m1:t key value) (m2:t key value).          {:pattern (equal m1 m2)}              equal m1 m2 <==> (forall k.{:pattern (sel m1 k); (sel m2 k)} sel m1 k == sel m2 k)
+assume SelConst:      forall (key:Type) (value:Type) (v:value) (k:key).                          {:pattern sel (const v) k}
+                      sel (const v) k == v
 
+assume SelRestrict:   forall (key:Type) (value:Type) (m:t key value) (ks:set key) (k:key).       {:pattern sel (restrict ks m) k}
+                      mem k ks ==> sel (restrict ks m) k == sel m k
 
-let const_on (key:Type) (value:Type) (dom:set key) (v:value) = restrict dom (const v) 
+assume SelConcat1:    forall (key:Type) (value:Type) (m1:t key value) (m2:t key value) (k:key).  {:pattern sel (concat m1 m2) k}
+                      contains m2 k ==> sel (concat m1 m2) k==sel m2 k
 
-opaque type DisjointDom (key:Type) (value:Type) (m1:t key value) (m2:t key value) = 
+assume SelConcat1:    forall (key:Type) (value:Type) (m1:t key value) (m2:t key value) (k:key).  {:pattern sel (concat m1 m2) k}
+                      not(contains m2 k) ==> sel (concat m1 m2) k==sel m1 k
+
+assume InDomUpd1:     forall (key:Type) (value:Type) (m:t key value) (k1:key) (k2:key) (v:value).   {:pattern contains (upd m k1 v) k2}
+                      contains (upd m k1 v) k2 == (k1=k2 || contains m k2)
+
+assume InDomUpd2:     forall (key:Type) (value:Type) (m:t key value) (k1:key) (k2:key) (v:value).{:pattern contains (upd m k2 v) k1}
+                      k2=!=k1 ==> contains (upd m k2 v) k1 == contains m k1
+
+assume InDomConstMap: forall (key:Type) (value:Type) (v:value) (k:key).                          {:pattern contains (const v) k}
+                      contains (const v) k
+
+assume InDomConcat:   forall (key:Type) (value:Type) (m1:t key value) (m2:t key value) (k:key).  {:pattern contains (concat m1 m2) k}
+                      contains (concat m1 m2) k==(contains m1 k || contains m2 k)
+
+assume InDomRestrict: forall (key:Type) (value:Type) (m:t key value) (ks:set key) (k:key).       {:pattern contains (restrict ks m) k}
+                      contains (restrict ks m) k == mem k ks
+
+assume ContainsConst: forall (key:Type) (value:Type) (v:value) (k:key).                          {:pattern contains (const v) k}
+                      not (contains (const v) k)
+
+assume Extensional:   forall (key:Type) (value:Type) (m1:t key value) (m2:t key value).          {:pattern (equal m1 m2)}
+                      equal m1 m2 <==> m1 == m2
+
+assume Equals:        forall (key:Type) (value:Type) (m1:t key value) (m2:t key value).          {:pattern (equal m1 m2)}
+                      equal m1 m2 <==> (forall k.{:pattern (sel m1 k); (sel m2 k)} sel m1 k == sel m2 k)
+
+let const_on (key:Type) (value:Type) (dom:set key) (v:value) = restrict dom (const v)
+
+opaque type DisjointDom (key:Type) (value:Type) (m1:t key value) (m2:t key value) =
           (forall x.{:pattern (contains m1 x)(* ; (contains m2 x) *)} contains m1 x ==> not (contains m2 x))
 
-module Set
-open Map
-type set (a:Type) = Map.t a bool
-let empty      (a:Type)                        = const a bool false
-let singleton  (a:Type) (x:a)                  = upd empty x true
-let mem        (a:Type) (x:a)      (s:set a)   = sel s x
-let union      (a:Type) (s1:set a) (s2:set a)  = concat s1 s2
-let intersect  (a:Type) (s1:set a) (s2:set a)  = intersect s1 s2
-let extend     (a:Type) (k:a)      (s:set a)   = upd s k true
-let complement (a:Type) (s:set a)              = complement s
-let minus      (a:Type) (s1:set a) (s2:set a)  = intersect s1 (complement s2)
-let equal      (a:Type) (s1:set a) (s2:set a)  = Map.equal s1 s2
-opaque type Subset' (a:Type) (s1:set a) (s2:set a) = (forall (x:a).{:pattern mem x s1} mem x s1 ==> mem x s2)
-type Subset : #a:Type -> set a -> set a -> Type = 
-    fun (a:Type) (s1:set a) (s2:set a) -> Subset' a s1 s2
 
 module Heap
 open Set
@@ -74,18 +119,62 @@ assume logic val equal:      heap -> heap -> Tot bool
 assume logic val restrict:   heap -> set aref -> Tot heap
 assume logic val concat:     heap -> heap -> Tot heap
 
-assume SelUpd1:       forall (a:Type) (h:heap) (r:ref a) (v:a).            {:pattern (sel (upd h r v) r)}       sel (upd h r v) r == v
-assume SelUpd2:       forall (a:Type) (h:heap) (k1:ref a) (k2:ref a) (v:a).{:pattern (sel (upd h k2 v) k1)}     k2=!=k1 ==> sel (upd h k2 v) k1 == sel h k1
-assume InDomUpd1:     forall (a:Type) (h:heap) (k:ref a) (v:a).            {:pattern contains (upd h k v) k}    contains (upd h k v) k
-assume InDomUpd2:     forall (a:Type) (h:heap) (k1:ref a) (k2:ref a) (v:a).{:pattern contains (upd h k2 v) k1}  k2=!=k1 ==> contains (upd h k2 v) k1 == contains h k1
-assume InDomEmp:      forall (a:Type) (k:ref a).                           {:pattern contains emp k}            not(contains emp k)
-assume Extensional:   forall (h1:heap) (h2:heap).                          {:pattern equal h1 h2}               equal h1 h2 <==> h1 == h2
-assume Equals:        forall (h1:heap) (h2:heap).                          {:pattern equal h1 h2}               equal h1 h2 <==> (forall (a:Type) (k:ref a).{:pattern (sel h1 k); (sel h2 k)} sel h1 k == sel h2 k)
-assume RestrictSel:   forall (a:Type) (h:heap) (r:set aref) (a:ref a).     {:pattern sel (restrict h r) a}      if b2t (mem (Ref a) r) then sel (restrict h r) a == sel h a else sel (restrict h r) a == sel emp a 
-assume RestrictIn:    forall (a:Type) (h:heap) (r:set aref) (a:ref a).     {:pattern contains (restrict h r) a} contains (restrict h r) a == (mem (Ref a) r && contains h a)
-assume SelConcat:     forall (a:Type) (h1:heap) (h2:heap) (a:ref a).       {:pattern sel (concat h1 h2) a}      if b2t (contains h2 a) then sel (concat h1 h2) a==sel h2 a else sel (concat h1 h2) a == sel h1 a
-assume ContainsConcat:forall (a:Type) (h1:heap) (h2:heap) (a:ref a).       {:pattern contains (concat h1 h2) a} contains h1 a || contains h2 a
+assume SelUpd1:       forall (a:Type) (h:heap) (r:ref a) (v:a).            {:pattern (sel (upd h r v) r)}       
+                      sel (upd h r v) r == v
+
+assume SelUpd2:       forall (a:Type) (b:Type) (h:heap) (k1:ref a) (k2:ref b) (v:b).{:pattern (sel (upd h k2 v) k1)}     
+                      k2=!=k1 ==> sel (upd h k2 v) k1 == sel h k1
+
+assume ContainsUpd:   forall (a:Type) (b:Type) (h:heap) (k1:ref a) (k2:ref b) (v:a).{:pattern contains (upd h k1 v) k2}
+                      contains (upd h k1 v) k2 <==> (k1==k2 \/ contains h k2)
+
+assume InDomEmp:      forall (a:Type) (k:ref a).                           {:pattern contains emp k}
+                      not(contains emp k)
+
+assume Extensional:   forall (h1:heap) (h2:heap).                          {:pattern equal h1 h2}               
+                      equal h1 h2 <==> h1 == h2
+
+assume Equals:        forall (h1:heap) (h2:heap).                          {:pattern equal h1 h2}               
+                      equal h1 h2 <==> (forall (a:Type) (k:ref a).{:pattern (sel h1 k); (sel h2 k)} sel h1 k == sel h2 k)
+
+assume RestrictSel:   forall (a:Type) (h:heap) (r:set aref) (a:ref a).     {:pattern sel (restrict h r) a}
+                      mem (Ref a) r ==> sel (restrict h r) a == sel h a
+
+assume RestrictIn:    forall (a:Type) (h:heap) (r:set aref) (a:ref a).     {:pattern contains (restrict h r) a}
+                      contains (restrict h r) a == (mem (Ref a) r && contains h a)
+
+assume SelConcat:     forall (a:Type) (h1:heap) (h2:heap) (a:ref a).       {:pattern sel (concat h1 h2) a}
+                      if b2t (contains h2 a) then sel (concat h1 h2) a==sel h2 a else sel (concat h1 h2) a == sel h1 a
+
+assume ContainsConcat:forall (a:Type) (h1:heap) (h2:heap) (a:ref a).       {:pattern contains (concat h1 h2) a}
+                      contains (concat h1 h2) a == (contains h1 a || contains h2 a)
 
 type On (r:set aref) (p:(heap -> Type)) (h:heap) = p (restrict h r)
 opaque type fresh (h:heap) (refs:set aref)       = (forall (a:Type) (a:ref a).{:pattern (contains h a)} mem (Ref a) refs ==> not(contains h a))
 
+
+assume val x : ref int
+assume val y : ref int
+assume val h : heap
+assume DistinctXY: x <> y
+
+let test0 _ = assert (sel (upd h x 0) x = 0)
+let test1 _ = assert (sel (upd (upd h x 0) y 1) x = 0)
+(* let test2 _ = assert (sel (upd (upd h x 0) y 1) y = 0) //should fail *)
+let test3 _ = assert (sel (upd (upd h x 0) y 1) y = 1)
+let h1 = upd (upd h x 0) y 1
+let test5 _ = assert (equal h1 (upd (upd h y 1) x 0))
+let ys = Set.singleton (Ref y)
+let test6 _ = assert (equal h1 (concat h1 (restrict h1 (complement ys))))
+let test7 _ = assert (contains h1 x)
+let test8 _ = assert (contains h y ==> contains (upd h x 0) y)
+let test9 (x:ref int) =
+  assume (not (contains h x));
+  assert (equal (upd h x 0) (concat (upd h x 0) (restrict h (complement empty))))
+
+(* let test10 (x:ref int) (y:ref int) (h0:heap) (h1:heap) (h2:heap) =  *)
+(*   admitP (h1 == concat h1 (restrict h0 (complement empty))) (); *)
+(*   admitP (h1 == upd h0 x 0) (); *)
+(*   admitP (~ (contains h1 y)) (); *)
+(*   assert false *)
+  
