examples/unit-tests/unit1.fst
@@ -87,7 +87,7 @@ let tabs_id ('a:Type) (x:'a) = x
 val id_pure_annot_eq : x:'a -> Pure 'a True (fun y -> y==x)
 let id_pure_annot_eq x = x
 
-val id_all_annot_eq: x:'a -> All 'a (fun h -> True) (fun h0 y h1 -> is_V y /\ h0==h1 /\ x==(V.v y)) (SomeRefs EmptySet)
+val id_all_annot_eq: x:'a -> All 'a (fun h -> True) (fun h0 y h1 -> is_V y /\ h0==h1 /\ x==(V.v y)) 
 let id_all_annot_eq x = x
 
 val hd: list 'a -> 'a
